README.md
@@ -2,7 +2,9 @@
 
 ```
 git submodule update --init
+rm -r _opam
 opam switch create ./ <ocaml version>
+git checkout _opam  # contains .ignore file for rg, fd, ...
 opam pin coq <coq version>
 opam repo add coq-released https://coq.inria.fr/opam/released
 opam repo add iris-dev https://gitlab.mpi-sws.org/iris/opam.git
